---
title: ARCH(1) process is a Markov process
date: 2020-07-29 02:13:00
categories:
- 笔记
- 博客园
tags:
- 博客园
- 搬家
- cnblogs
---
# [这是👉ARCH(1) process is a Markov process👈的摘要](../../../../2020/07/29/cnblog_13395527/)
<!--more-->
**------------恢复内容开始------------** I have a question about the ARCH(1)
process. Let $(\Omega, \mathcal F, P)$ be a probability space, let $(Z_t)_{t
\in \mathbb Z}$ be a sequence of i.i.d. real-valued random variables with mean
zero and variance one. A stochastic process $(X_t)_{t \in \mathbb Z}$ is an
ARCH(1)-process if it is strictly stationary and if, for all $t$ and some
process $(\sigma_t)$ with $\sigma_t > 0$ for every $t$, one has $X_t =
\sigma_t Z_t$ and $\sigma_t^2 = \alpha_0 + \alpha_1 X_{t-1}^2$, where
$\alpha_0 > 0$ and $\alpha_1 \ge 0$. Let $\mathcal F_t$ be the natural
filtration of the process $(X_t)$, i.e. $\mathcal F_t = \sigma(X_s; s \le t)$.
I want to prove that $(X_t)$ has the Markov property, i.e. for each $B \in
\mathcal B(\mathbb R)$ and for all $s, t \in\mathbb Z$ with $s < t$, one has
$P[X_t \in B \mid \mathcal F_s] = P[X_t \in B \mid X_s]$. Is that possible?
##ANswer For s < t we can write: $$X_t = Z_t \sqrt{\alpha_0 +
\alpha_1X_{t-1}^2} = Z_t \sqrt{\alpha_0 + \alpha_0\alpha_1 Z_{t-1}^2 +
\alpha_1^2Z_{t-1}^2X_{t-1}^2}\\\ = \ldots = Z_t \sqrt{\sum_{k = 0}^{t-s-1}
\alpha_0 \alpha_1^k\prod_{i=1}^k Z_{t-i}^2 + \alpha_1^{t-s}\prod_{i=1}^{t-s}
Z_{t-i}^2 X_{s}^2}$$ By construction $Z_t,\ldots, Z_{s+1}$ is independent to
$\mathcal{F}_s$, so for a measureable function $g \geq 0$ it holds:
$$\Bbb{E}[g(X_t) | \mathcal{F}_s ] = \Bbb{E}\left[g\left(Z_t \sqrt{\sum_{k =
0}^{t-s-1} \alpha_0 \alpha_1^k\prod_{i=1}^k Z_{t-i}^2 +
\alpha_1^{t-s}\prod_{i=1}^{t-s} Z_{t-i}^2 X_{s}^2} \right) \Big| \mathcal{F}_s
\right] \\\ = \Bbb{E}\left[g\left(Z_t \sqrt{\sum_{k = 0}^{t-s-1} \alpha_0
\alpha_1^k\prod_{i=1}^k Z_{t-i}^2 + \alpha_1^{t-s}\prod_{i=1}^{t-s} Z_{t-i}^2
x^2} \right) \right]_{x = X_s} = \Bbb{E}[g(X_t) | X_s ]$$ Here the notation $x
= X_s$ denotes that we don't integrate over $X_s$ anymore, but set the value
of $x$ in the expection by evaluating $X_s$ first. In the last step we just go
back the steps before but with $\sigma$-Algebra $X_s$. This shows $\Bbb{P}[X_t
\in B | \mathcal{F}_s] = \Bbb{P}[X_t \in B | X_s]$, but it is not the full
Markov property. For the Markov property you need additionally $\Bbb{P}[X_t
\in B | X_s] = \Bbb{P}[X_{t-s} \in B | X_0 = x]_{x= X_s}$, but this follow
from the calculations above, because the $Z_t$ are i.i.d.
**------------恢复内容结束------------**


